compiler/pollang/PolLang.v
@@ -5,55 +5,55 @@ Require Import List.
 
 Section PolLang.
 
-Variable NB_MSG:nat.
-Variable PLT:vvdesc NB_MSG.
+Context {NB_MSG:nat}.
+Variable PAYD:vvdesc NB_MSG.
 
 (*after occurs immediately after before occurs.*)
-Inductive ImmAfter (after:@KOAction NB_MSG PLT) (before:@KOAction NB_MSG PLT)
-  : @KTrace NB_MSG PLT -> Prop :=
+Inductive ImmAfter (after:KOAction PAYD) (before:KOAction PAYD)
+  : KTrace PAYD -> Prop :=
 | IA_nil : ImmAfter after before nil
 (*An action not matching before is added*)
 | IA_nB : forall before' tr, ImmAfter after before tr ->
-                             ~AMatch before before' ->
+                             ~AMatch PAYD before before' ->
                              ImmAfter after before (before'::tr)
 (*An action matching before is added*)
 | IA_B : forall before' after' tr, ImmAfter after before tr ->
-                                   AMatch after after' ->
+                                   AMatch PAYD after after' ->
                                    ImmAfter after before (after'::before'::tr).
 
 (*before occurs immediate before after occurs*)
-Inductive ImmBefore (before:@KOAction NB_MSG PLT) (after:@KOAction NB_MSG PLT)
-  : @KTrace NB_MSG PLT -> Prop :=
+Inductive ImmBefore (before:KOAction PAYD) (after:KOAction PAYD)
+  : KTrace PAYD -> Prop :=
 | IB_nil : ImmBefore before after nil
 (*An action not matching after is added*)
 | IB_nA : forall after' tr, ImmBefore before after tr ->
-                            ~AMatch after after' ->
+                            ~AMatch PAYD after after' ->
                             ImmBefore before after (after'::tr)
 (*An action matching after is added*)
 | IB_A : forall after' before' tr, ImmBefore before after tr ->
-                                   AMatch before before' ->
+                                   AMatch PAYD before before' ->
                                    ImmBefore before after (after'::before'::tr).
 
-Inductive Release (past:@KOAction NB_MSG PLT) (future:@KOAction NB_MSG PLT)
-  : @KTrace NB_MSG PLT -> Prop :=
+Inductive Release (past:KOAction PAYD) (future:KOAction PAYD)
+  : KTrace PAYD -> Prop :=
 | R_nil : Release past future nil
 | R_not_future : forall act tr, Release past future tr ->
-                                ~AMatch future act ->
+                                ~AMatch PAYD future act ->
                                 Release past future (act::tr)
 | R_future : forall act tr, Release past future tr ->
                             (exists past', In past' tr /\
-                                           AMatch past past') ->
+                                           AMatch PAYD past past') ->
                             Release past future (act::tr).
 
-Inductive Disables (disabler:@KOAction NB_MSG PLT) (disablee:@KOAction NB_MSG PLT)
-  : @KTrace NB_MSG PLT -> Prop :=
+Inductive Disables (disabler:KOAction PAYD) (disablee:KOAction PAYD)
+  : KTrace PAYD -> Prop :=
 | D_nil : Disables disabler disablee nil
 | D_not_disablee : forall act tr, Disables disabler disablee tr ->
-                                  ~AMatch disablee act ->
+                                  ~AMatch PAYD disablee act ->
                                   Disables disabler disablee (act::tr)
 | D_disablee : forall act tr, Disables disabler disablee tr ->
                               (forall act', In act' tr ->
-                                            ~AMatch disabler act') ->
+                                            ~AMatch PAYD disabler act') ->
                               Disables disabler disablee (act::tr).
 
 End PolLang.
