compiler/pollang/EchoPolicies.v
@@ -6,12 +6,12 @@ Require Import Tactics.
 
 Theorem recv_before : forall st tr m,
   Reach _ _ COMPS _ _ INIT HANDLERS st -> ktr _ _ st = inhabits tr ->
-  ImmBefore NB_MSG PAYD
-            (@KORecv NB_MSG PAYD None
-                     (Some (@Build_opt_msg NB_MSG PAYD
+  ImmBefore PAYD
+            (KORecv PAYD None
+                     (Some (Build_opt_msg PAYD
                                            None (Some m, tt))))
-            (@KOSend NB_MSG PAYD None
-                     (Some (@Build_opt_msg NB_MSG PAYD
+            (KOSend PAYD None
+                     (Some (Build_opt_msg PAYD
                                            None (Some m, tt))))
             tr.
 Proof.
@@ -20,12 +20,12 @@ Qed.
 
 Theorem send_after : forall st tr m,
   Reach _ _ COMPS _ _ INIT HANDLERS st -> ktr _ _ st = inhabits tr ->
-  ImmAfter NB_MSG PAYD
-            (@KOSend NB_MSG PAYD None
-                     (Some (@Build_opt_msg NB_MSG PAYD
+  ImmAfter PAYD
+            (KOSend PAYD None
+                     (Some (Build_opt_msg PAYD
                                            None (Some m, tt))))
-            (@KORecv NB_MSG PAYD None
-                     (Some (@Build_opt_msg NB_MSG PAYD
+            (KORecv PAYD None
+                     (Some (Build_opt_msg PAYD
                                            None (Some m, tt))))
             tr.
 Proof.
