compiler/pollang/ReflexKState.v
@@ -78,12 +78,12 @@ Require Import Ynot.
 
 Theorem release : forall st tr u,
   Reach _ _ COMPS _ _ INIT HANDLERS st -> ktr _ _ st = inhabits tr ->
-  Release NB_MSG PAYD
-          (@KORecv NB_MSG PAYD None
-                   (Some (@Build_opt_msg NB_MSG PAYD
+  Release PAYD
+          (KORecv PAYD None
+                   (Some (Build_opt_msg PAYD
                                          (Some None) (Some u, (None, tt)))))
-          (@KOSend NB_MSG PAYD None
-                   (Some (@Build_opt_msg NB_MSG PAYD
+          (KOSend PAYD None
+                   (Some (Build_opt_msg PAYD
                                          None (Some u, tt))))
           tr.
 Proof.
